\documentclass[12pt, a4paper]{article}

\usepackage[a4paper, margin=1in]{geometry}

\input{preamble}
\input{letterfonts}
\newcommand{\mytitle}{MA1521 Homework 8}
\newcommand{\myauthor}{github/omgeta}
\newcommand{\mydate}{AY 24/25 Sem 1}

\begin{document}
\raggedright
\footnotesize
\begin{center}
{\normalsize{\textbf{\mytitle}}} \\
{\footnotesize{\mydate\hspace{2pt}\textemdash\hspace{2pt}\myauthor}}
\end{center}
\setlist{topsep=-1em, itemsep=-1em, parsep=2em}

%%%%%%%%%%%%%%%%%%%%%%%%%%%%%%%%%%%%%%%%%%%%%%%%%%%%%%
%                      Begin                         %
%%%%%%%%%%%%%%%%%%%%%%%%%%%%%%%%%%%%%%%%%%%%%%%%%%%%%%
\begin{enumerate}[Q\arabic*.]
  \item 
    \begin{enumerate}[(\alph*)]
      \item $\displaystyle f(x, y) = \frac{x^2}{y^2+2} - \frac{y^2}{x^2+y}$
        \begin{align*}
          \frac{\partial f}{\partial x} &= \frac{(y^2+2)(2x) - (x^2)(0)}{(y^2+2)^2} - \frac{(x^2+y)(0) - (y^2)(2x)}{(x^2+y)^2} \\
                                        &= \frac{2x}{y^2 + 2} + \frac{2xy^2}{(x^2+y)^2}\qed\\
          \frac{\partial f}{\partial y} &= \frac{(y^2+2)(0) - (x^2)(2y)}{(y^2+2)^2} - \frac{(x^2+y)(2y) - (y^2)(1)}{(x^2+y)^2}\\
                                        &= \frac{-2yx^2}{(y^2+2)^2} - \frac{2yx^2+y^2}{(x^2+y)^2} \qed
        \end{align*}

      \item $\displaystyle g(x,y,z) = xy^2z^3 + 3yz + \ln(z^2+1)$
        \begin{align*}
          \frac{\partial g}{\partial x} &= y^2z^3 \qed\\
          \frac{\partial g}{\partial y} &= 2xyz^3 + 3z \qed\\
          \frac{\partial g}{\partial z} &= 3xy^2z^2 + 3y + \frac{2z}{z^2+1} \qed
        \end{align*}
    \end{enumerate}

  \item $f(x, y) = e^xy^2 + x\sin xy$
    \begin{align*}
      f_x &= e^xy^2 + \sin xy + xy \cos xy \qed\\
      f_y &= 2e^xy + x^2\cos xy \qed\\
      f_{xy} &= \frac{\partial}{\partial y} f_x \\
             &= 2e^xy + x\cos xy + x\cos xy - x^2y\sin xy\\
             &= 2e^xy + 2x\cos xy - x^2y\sin xy \qed
    \end{align*}

  \item $f(x,y,z) = e^{xy^2} + x^2 + \sin^{-1} y$
    \begin{align*}
      f_x &= y^2e^{xy^2} + 2x\\
      f_{xx} &= y^4e^{xy^2} + 2\\
      f_{xxy} &= 2xy^5e^{xy^2} + 4y^3e^{xy^2}\\
              &= 2y^3e^{xy^2}(xy^2 + 2)\qed
    \end{align*}

  \item $x^3 + 2y^3 + 6xz^3 = 61z$\\
    Differentiate w.r.t. $x$:
    \begin{align*}
      3x^2 + 6z^3 + 18xz^2 \frac{\partial z}{\partial x} &= 61 \frac{\partial z}{\partial x}\\
      \frac{\partial z}{\partial x} &= \frac{3x^2 + 6z^3}{61 - 18xz^2} \qed
    \end{align*}
    Differentiate w.r.t. $y$:
    \begin{align*}
      6y^2 + 18xz^2 \frac{\partial z}{\partial y} &= 61 \frac{\partial z}{\partial y}\\
      \frac{\partial z}{\partial y} &= \frac{6y^2}{61-18xz^2} \qed
    \end{align*}

  \pagebreak
  \item 
    \begin{enumerate}[(\alph*)]
      \item $I = 7V \implies \frac{dI}{dV} = 7 \text{ (dollars per day per thousand views)}$ \qed
      \item When $300 = V \times R \implies R = \frac{300}{V}$:
        \begin{align*}
          \frac{dR}{dV} &= -\frac{300}{V^2}\\
          \frac{dR}{dV}|_{V=50} &= -0.12\text{ (dollars per thousand views per thousands of view per day)}\qed
        \end{align*}
      \item Differentiate w.r.t. $t$:
        \begin{align*}
          \frac{dI}{dt} &= \frac{dV}{dt}R + \frac{dR}{dt}V
        \end{align*}
        Substitute $R = 5, V = 70, \frac{dR}{dt} = 0.02, \frac{dI}{dt} = 8$:
        \begin{align*}
          8 &= 5\frac{dV}{dt} + (0.02)(70)\\
          \frac{dV}{dt} &= 1.32\text{ (thousands of views per day per day)} \qed
        \end{align*}
    \end{enumerate}

  \item 
    \begin{enumerate}[(\alph*)]
      \item At $\displaystyle (-1,1,-\frac{1}{6})$: 
        \begin{align*}
          \frac{\partial z}{\partial x} &= -\frac{7}{6}\\
          \frac{\partial z}{\partial y} &= -\frac{35}{36}\\
          \text{Tangent: }z+\frac{1}{6} &= -\frac{7}{6}(x+1) - \frac{35}{36}(y-1)\\
          z &= -\frac{7}{6}x -\frac{35}{36}y-\frac{13}{36}\qed
        \end{align*}
      \item At $(3, 2, 1)$:
        \begin{align*}
          \frac{\partial z}{\partial x} &= \frac{33}{7}\\
          \frac{\partial z}{\partial y} &= \frac{24}{7}\\
          \text{Tangent: }z-1 &= \frac{33}{7}(x-3) + \frac{24}{7}(y-2)\\
           z &= \frac{33}{7}x + \frac{24}{7}y - 20 \qed
        \end{align*}
    \end{enumerate}
\end{enumerate}
%%%%%%%%%%%%%%%%%%%%%%%%%%%%%%%%%%%%%%%%%%%%%%%%%%%%%%
%                       End                          %
%%%%%%%%%%%%%%%%%%%%%%%%%%%%%%%%%%%%%%%%%%%%%%%%%%%%%%

\end{document}
