\documentclass[12pt, a4paper]{article}

\usepackage[a4paper, margin=1in]{geometry}

\input{preamble}
\input{letterfonts}
\newcommand{\mytitle}{MA1521 Homework 5}
\newcommand{\myauthor}{github/omgeta}
\newcommand{\mydate}{AY 24/25 Sem 1}

\begin{document}
\raggedright
\footnotesize
\begin{center}
{\normalsize{\textbf{\mytitle}}} \\
{\footnotesize{\mydate\hspace{2pt}\textemdash\hspace{2pt}\myauthor}}
\end{center}
\setlist{topsep=-1em, itemsep=-1em, parsep=2em}

%%%%%%%%%%%%%%%%%%%%%%%%%%%%%%%%%%%%%%%%%%%%%%%%%%%%%%
%                      Begin                         %
%%%%%%%%%%%%%%%%%%%%%%%%%%%%%%%%%%%%%%%%%%%%%%%%%%%%%%
\begin{enumerate}[Q\arabic*.]
  \item 
    \begin{enumerate}[(\alph*)]
      \item 
        \begin{align*}
          \text{Area} &= \int^{\pi/3}_{-\pi/3} \frac{1}{2}\sec^2x + 4\sin^2x dx\\
                      &= \int^{\pi/3}_{-\pi/3} \frac{1}{2}\sec^2x + 2 - 2\cos2x dx\\
                      &= [\frac{1}{2}\tan x + 2x - \sin 2x]^{\pi/3}_{-\pi/3}\\
                      &= (\frac{1}{2}\tan \frac{\pi}{3} + \frac{2\pi}{3} - \sin \frac{2\pi}{3}) - (\frac{1}{2}\tan -\frac{\pi}{3} - \frac{2\pi}{3} - \sin -\frac{2\pi}{3})\\
                      &= (\frac{\sqrt{3}}{2} + \frac{2\pi}{3} - \frac{\sqrt{3}}{2}) - (-\frac{\sqrt{3}}{2} - \frac{2\pi}{3} + \frac{\sqrt{3}}{2})\\
                      &= \frac{4\pi}{3} \qed
        \end{align*}

      \item Express $y=\frac{1}{4}x^2$ in terms of $y$: $x = \pm2\sqrt{y}$\\
        Express $y=x$ in terms of $y$: $x = y$
        \begin{align*}
          \text{Area} &= \int^1_0 2\sqrt{y} - y dy\\
                      &= [\frac{4}{3}y^{\frac{3}{2}} -\frac{y^2}{2}]^1_0\\
                      &= (\frac{4}{3} - \frac{1}{2}) - (0 - 0)\\
                      &= \frac{5}{6}\qed
        \end{align*}

      \item Graphs of $y=4-x^2$ and $y=2-x$ intersect at: 
        \begin{align*}
          4-x^2 &= 2-x\\
          x^2-x-2 &= 0\\
          (x-2)(x+1) &= 0\\
          x = -1, 2
        \end{align*}
        Then, find the area:
        \begin{align*}
          \text{Area} &= \int^{-1}_{-2} (2-x)-(4-x^2)dx +\int^2_{-1}(4-x^2)-(2-x)dx\\
                      &= \int^{-1}_{-2} x^2-x-2 dx + \int^{2}_{-1} 2 + x -x^2 dx\\
                      &= [\frac{x^3}{3} - \frac{x^2}{2}-2x]^{-1}_{-2} + [2x+\frac{x^2}{2}-\frac{x^3}{3}]^2_{-1}\\
                      &= (-\frac{1}{3} -\frac{1}{2} + 2) - (-\frac{8}{3} -2 + 4) + (4 + 2 -\frac{8}{3}) - (-2 + \frac{1}{2} + \frac{1}{3})\\
                      &= \frac{19}{3} \qed
        \end{align*}
    \end{enumerate}
    \pagebreak

  \item 
    \begin{enumerate}[(\alph*)]
      \item First, find the derivative:
        \begin{align*}
          y &= \ln(\sec x)\\
          \frac{dy}{dx} &= \frac{\sec x \tan x }{\sec x}\\
                        &= \tan x 
        \end{align*}
        Then, find the arc length:
        \begin{align*}
          \text{Arc length} &= \int^{\pi/4}_0 \sqrt{1 + \tan^2x}dx\\
          &= \int^{\pi /4}_0 \sec x dx\\
          &= [\ln(\sec x + \tan x)]^{\pi /4}_0\\
          &= \ln(\sqrt{2} + 1) - \ln(1 + 0)\\
          &= \ln(\sqrt{2} + 1)\qed
        \end{align*}

      \item First, find the derivative:
        \begin{align*}
          x &= \frac{1}{2}e^{2y} + \frac{1}{8}e^{-2y}\\
          \frac{dx}{dy} &= e^{2y} - \frac{1}{4}e^{-2y}
        \end{align*}
        Then, find the arc length:
        \begin{align*}
          \text{Arc length} &= \int^{\ln 3}_{\ln 2} \sqrt{1 + (e^{2y} - \frac{1}{4}e^{-2y})^2} dy\\
                            &= \int^{\ln 3}_{\ln 2} \sqrt{1 + e^{4y} +\frac{1}{16}e^{-4y} - \frac{1}{2}} dy\\
                            &= \int^{\ln 3}_{\ln 2} \sqrt{e^{4y} +\frac{1}{2}+\frac{1}{16}e^{-4y}} dy\\
                            &= \int^{\ln 3}_{\ln 2} \sqrt{(e^{2y} + \frac{1}{4}e^{-2y})^2} dy\\
                            &= \int^{\ln 3}_{\ln 2} e^{2y} + \frac{1}{4}e^{-2y} dy\\
                            &= [\frac{e^{2y}}{2} - \frac{1}{8}e^{-2y}]^{\ln 3}_{\ln 2}\\
                            &= (\frac{e^{2\ln 3}}{2} - \frac{e^{-2\ln 3}}{8}) - (\frac{e^{2\ln 2}}{2} - \frac{e^{-2\ln 2}}{8})\\
                            &= (\frac{3^2}{2} - \frac{3^{-2}}{8}) - (\frac{2^2}{2} - \frac{2^{-2}}{8})\\
                            &= \frac{725}{288} \qed
        \end{align*}
    \end{enumerate}
    \pagebreak
  \item 
    \begin{align*}
      \text{Volume} &= \pi\int^1_0 x^2 dx + \pi\int^2_1 4x^2-4x+1 dx\\
                    &= \pi[\frac{x^3}{3}]^1_0 + \pi[\frac{4}{3}x^3 - 2x^2 + x]^2_1\\
                    &= \pi(\frac{1}{3}) + \pi(\frac{14}{3} - \frac{1}{3})\\
                    &= \frac{14\pi}{3}\qed
    \end{align*}

  \item Curves $x = y^2+1$ and $x=3$ intersect at:
    \begin{align*}
      y^2 + 1 &= 3\\
      y^2 = 2\\
      y = \pm\sqrt{2}
    \end{align*}
    Then, find the volume:
    \begin{align*}
      \text{Volume} &= \pi\int^{\sqrt{2}}_{-\sqrt{2}}(3 - (y^2 + 1))^2 dy\\
                    &= \pi\int^{\sqrt{2}}_{-\sqrt{2}}(2-y^2)^2 dy\\
                    &= \pi\int^{\sqrt{2}}_{-\sqrt{2}} 4- 4y^2 + y^4 dy\\
                    &= \pi[4y - \frac{4}{3}y^3 + \frac{1}{5}y^5]^{\sqrt{2}}_{-\sqrt{2}}\\
                    &= \pi[(4\sqrt{2} - \frac{4}{3}(2\sqrt{2}) + \frac{1}{5}(4\sqrt{2})) \\&- (-4\sqrt{2} +\frac{4}{3}(2\sqrt{2}) -\frac{1}{5}(4\sqrt{2}))]\\
                    &= \pi(8\sqrt{2}-\frac{16}{3}\sqrt{2}+\frac{8}{5}\sqrt{2})\\
                    &= \frac{64}{15}\sqrt{2}\pi\qed
    \end{align*}
  \pagebreak
  \item Curves $y=\sqrt{x-1}$ and $y=(x-1)^2$ intersect at:
    \begin{align*}
      (x-1)^2 &= \sqrt{x-1}\\
      (x-1)^4 &= x-1\\
      u^4 &= u\tag*{(Sub $u=x-1$)}\\
      u(u^3-1) &= 0\\
      u &= 0, 1\\
      \therefore x &= 1, 2
    \end{align*}
    Then, find the volume:
    \begin{align*}
      \text{Volume} &= 2\pi \int^2_1 x|\sqrt{x-1}-(x-1)^2|dx\\
                    &= 2\pi(\int^2_1x\sqrt{x-1}dx - \int^2_1x(x-1)^2dx)\\
                    &= 2\pi(\int^1_0(u+1)\sqrt{u}du - \int^2_1x^3-2x^2+x dx)\tag*{(Sub $u = x-1$)}\\
                    &= 2\pi(\int^1_0u^{3/2}+u^{1/2}du - [\frac{x^4}{4} - \frac{2x^3}{3}+\frac{x^2}{2}]^2_1)\\
                    &= 2\pi([\frac{2}{5}u^{5/2} + \frac{2}{3}u^{3/2}]^1_0 - (\frac{2}{3} - \frac{1}{12}))\\
                    &= 2\pi[(\frac{16}{15}) - (\frac{7}{12})]\\
                    &= 2\pi(\frac{29}{60})\\
                    &= \frac{29}{30}\pi \qed
    \end{align*}
\end{enumerate}
%%%%%%%%%%%%%%%%%%%%%%%%%%%%%%%%%%%%%%%%%%%%%%%%%%%%%%
%                       End                          %
%%%%%%%%%%%%%%%%%%%%%%%%%%%%%%%%%%%%%%%%%%%%%%%%%%%%%%

\end{document}
